src/playground/generated_codes/find_shared_element.dfy
@@ -1,0 +1,19 @@
+method FindSharedElements(arr1: array<int>, arr2: array<int>) returns (shared: array<int>)
+{
+  var temp: seq<int> := [];
+  for i: int := 0 to arr1.Length - 1
+  {
+    for j: int := 0 to arr2.Length - 1
+    {
+      if arr1[i] == arr2[j] && !temp.Contains(arr1[i])
+      {
+        temp := temp + [arr1[i]];
+      }
+    }
+  }
+  shared := new int[temp.Length];
+  for k: int := 0 to temp.Length - 1
+  {
+    shared[k] := temp[k];
+  }
+}
