src/tests/dafny/copyArray.dfy
@@ -12,3 +12,4 @@ method CopyArray(source: array<int>, destination: array<int>)
     n := n + 1;
   }
 }
+
